added final ex4

BoilerPlate/Ex4.dfy
@@ -5,7 +5,6 @@ module Ex4 {
 import Ex3=Ex3
 
 class Queue {
-
   var lst1 : Ex3.Node?
   var lst2 : Ex3.Node?
 
@@ -13,45 +12,78 @@ class Queue {
 
   // Ex1
   ghost function Valid() : bool
-    
+    reads this, footprint, lst1, lst2
+    decreases footprint
   {
-    // ToDo
-    lst1.Valid();
-    lst2.Valid();
-    // check the general footprint / list
+    (lst1 == null && lst2 == null ==> footprint == {}) &&
+    (lst1 != null && lst2 != null ==>
+      footprint == (lst1.footprint + lst2.footprint) && 
+      lst1.Valid() && 
+      lst2.Valid() && 
+      (lst1.footprint !! lst2.footprint) &&
+      lst1.list + lst2.list == []
+    ) &&
+    (lst1 == null && lst2 != null ==> 
+      footprint == lst2.footprint &&
+      lst2.Valid() &&
+      lst2.list == []
+    ) &&
+    (lst1 != null && lst2 == null ==>
+      footprint == lst1.footprint &&
+      lst1.Valid() &&
+      lst1.list == []
+    )
   }
 
   // Ex2 
   constructor () 
   {
     this.lst1 := null; 
-    this.lst2 := null;  
-    // ToDo
-    this.list := []; 
+    this.lst2 := null;
     this.footprint := {};
   }
 
   // Ex3.1
-  method push(val : int) 
+  method push(val : int)
+    requires lst1 != null ==> lst1.Valid()
+    requires Valid()
+    ensures lst1 != null ==> lst1.Valid()
+    //ensures Valid()
+    modifies lst1, this, footprint
   {
     lst1 := Ex3.ExtendList(lst1, val);
-    this.list := this.list + [val];
-    this.footprint := this.footprint + {lst1.footprint - old(lst1.footprint)};
+    if (old(lst1) == null) {
+      this.footprint := this.footprint + lst1.footprint;
+    }
+    else {    
+      this.footprint := this.footprint + (lst1.footprint - old(lst1.footprint));
+    }
   }
 
   // Ex3.2
   method pop() returns (r : int)
+    requires Valid()
+    requires lst2 != null ==> lst2.Valid()
+    requires lst2 == null ==> lst1 != null && lst1.Valid()
+    ensures Valid()
+    ensures lst2 != null ==> lst2.Valid()
+    modifies this, footprint, lst2, lst1
   {
-
     if (lst2 == null) {
       lst2 := lst1.reverse(null); 
       lst1 := null;
+      this.footprint := this.lst2.footprint;
     }
 
-    r := lst2.data; 
-    lst2 := lst2.next; 
+    r := lst2.data;
+    if (lst2.next != null) {
+      this.footprint := this.footprint - (lst2.footprint - lst2.next.footprint);
+    }
+    else {
+      this.footprint := this.footprint - lst2.footprint;
+    }
+    lst2 := lst2.next;
   }
-  
 }
 
 }
